\documentclass{article}
\usepackage{amsmath, amssymb, amsthm, sectsty}

\begin{document}
	
	\textbf{Sum Law}
	
	\section*{Claim: $\lim_{x \to a} f(x)^n = M^n$}
	
	
	\begin{proof}
		
		Provided that $\lim_{x \to c} f(x) = M, \quad \lim_{x \to c} g(x) = N, \quad \text{and } N \neq 0.$ Using the $\varepsilon$â€“$\delta$ definition of a limit, we will prove by induction that for all n $\in \mathbb{N}$:
		\[
		\lim_{x \to a} f(x)^n = M^n
		\]
		
		The definition tell us, that for every $\varepsilon > 0$, there exists a $\delta > 0$ such that if $0 < |x - a| < \delta$, then $|f(x) - L| < \varepsilon$.
		
		
		Suppose $0 < |x - a| < \delta$. In a base case of $n = 1$:
		\[
		|f(x)^1 - M^1| = |f(x) - M|
		\]
		
		Now suppose $|x - a| < \delta$, it follows that:
		\[
		|f(x) - M| < \epsilon
		\]
		
		Hence, the base case of $n = 1$ holds.
		
		\vspace{1cm}
		
		Assume $\lim_{x \to a} f(x)^n = M^n$ holds for all $n \in \mathbb{N}$.
		
		Now suppose $|x - a| < \delta$, it follows that:
		\[
		|f(x)^n - M^n| < \epsilon
		\]
		
		Using this assumption, we must show that \( \lim_{x \to a} f(x)^{n+1} = M^{n+1} \) holds as well.
		
		Let us first analyse the distance between the function and its limit point:
		
		\[
		|f(x)^{n+1} - M^{n+1}| 
		= |f(x) \cdot f(x)^n - M \cdot M^n|
		\]
		
		\[
		= |f(x) \cdot f(x)^n - f(x) \cdot M^n + f(x) \cdot M^n - M \cdot M^n|
		\]
		
		\[
		= |f(x)(f(x)^n - M^n) + M^n(f(x) - M)|
		\]
		
		Now apply the triangle inequality:
		
		\[
		\leq |f(x)| \cdot |f(x)^n - M^n| + |M^n| \cdot |f(x) - M|
		\]
		
		Such that:
		\[
		|f(x)| \cdot |f(x)^n - M^n| < \frac{\epsilon}{2}
		\]
		\[
		|M^n| \cdot |f(x) - M| < \frac{\epsilon}{2}
		\]
		
		Since \( |f(x) - M| < \epsilon_1 \) whenever \( |x - a| < \delta_1 \), and
		\( |f(x)^n - M^n| < \epsilon_2 \) whenever \( |x - a| < \delta_2 \),  
		choose
		\[
		\delta = \min(\delta_1, \delta_2)
		\]
		
		Then, for all \( x \) such that \( 0 < |x - a| < \delta \), we have:
		\[
		|f(x)^{n+1} - M^{n+1}| 
		\leq |f(x)| \cdot |f(x)^n - M^n| + |M^n| \cdot |f(x) - M|
		< |f(x)| \cdot \epsilon_2 + |M^n| \cdot \epsilon_1
		\]
		
		Now choose \( \epsilon_1 = \frac{\epsilon}{2|M^n|} \)  
		and \( \epsilon_2 = \frac{\epsilon}{2|f(x)|} \)  
		so the total is less than \( \epsilon \).
		
		Hence, the formula holds for \( n+1 \).
		
		
		
		
		
		
		
		
		
		
		
		
		
		
		
		
		
		
		
		
		
		
		
		
		
		
		
		
		
		
		
		
	\end{proof}
	
\end{document}