\documentclass{article}
\usepackage{amsmath, amssymb, amsthm, sectsty}

\begin{document}

\textbf{Sum Law}

\section*{Claim: $\lim_{x \to a} [f(x) - g(x)] = M - N$}


\begin{proof}

Provided that $\lim_{x \to c} f(x) = M, \quad \lim_{x \to c} g(x) = N, \quad \text{and } N \neq 0.$ Using the $\varepsilon$â€“$\delta$ definition of a limit, we will directly prove that:
\[
\lim_{x \to c} \frac{f(x)}{g(x)} = \frac{M}{N}
\]


The definition tell us, that for every $\varepsilon > 0$, there exists a $\delta > 0$ such that if $0 < |x - a| < \delta$, then $|f(x) - L| < \varepsilon$.

Suppose $0 < |x - a| < \delta$. Let us analyze the distance between the function and its limit value:
\[
|f(x)/g(x) - M/N| = |f(x)(N - M) + M(f(x) - g(x)| / |g(x)N|
\]

Then using the triangle inequality, we can estimate each part as follows:
\[
\left| \frac{f(x)(N - M) + M(f(x) - g(x))}{g(x)N} \right|
\leq \frac{|f(x)||N - M| + |M||f(x) - g(x)|}{|g(x)N|}
\]

Hence, for every $\varepsilon > 0$, there exists a $\delta > 0$ such that if $0 < |x - c| < \delta$, then $|f(x) - g(x) - (M - N)| < \varepsilon$. Thus, we can conclude:
\[
\lim_{x \to c} [f(x) - g(x)] = M - N.
\]

To put a lower bound on $|g(x)|$, choose $\delta_1 = \frac{|N|^2}{2}$ such that if $|g(x) - N| < \delta_1$, then:
\[
|g(x)||N| > \frac{|N|^2}{2}
\quad \Rightarrow \quad
\frac{1}{|g(x)||N|} < \frac{2}{|N|^2}
\]

Then we can represent the total as:
\[
\frac{|f(x)||N - M| + |M||f(x) - g(x)|}{|g(x)||N|}
< \left( |f(x)||N - M| + |M||f(x) - g(x)| \right) \cdot \frac{2}{|N|^2}
< \epsilon
\]

Since the total expression is to be bounded by $\epsilon$, choose $\delta_2 = \frac{\epsilon |N|}{4}$. We can bound each part individually as follows:
\[
|f(x)||N - M| < \frac{\epsilon |N|}{4}
\quad \text{and} \quad
|M||f(x) - g(x)| < \frac{\epsilon |N|}{4}
\]

Bounding $|f(x)|$, choose $\delta_3 = 1 + |L|$ such that:
\[
|f(x)| < 1 + |L|
\]

Since $|f(x)|$ is bounded. Choose $\delta_4 = e|N|/4(1 + |L|)$, it follows that:
\[
|f(x)||N - M| < \frac{\epsilon |N|}{4} 
\quad \Rightarrow \quad
|N - M| < \frac{\epsilon |N|}{4(1 + |L|)}
\]


Now choose $
\delta = \min \left(
\frac{2}{|N|}, \quad
\frac{\epsilon |N|}{4|M|}, \quad
1 + |L|, \quad
\frac{\epsilon |N|}{4(1 + |L|)}
\right) $ such that:

\[
\frac{|f(x)||N - M| + |M||f(x) - g(x)|}{|g(x)N|}
< \left[
(1 + |L|) \cdot \frac{\epsilon |N|}{4(1 + |L|)} \; + \; |M| \cdot \frac{\epsilon |N|}{4|M|}
\right] \cdot \frac{2}{|N|}
\]

Simplifying the right side:

\[
= \left[ \frac{\epsilon |N|}{4} + \frac{\epsilon |N|}{4} \right] \cdot \frac{2}{|N|}
= \frac{\epsilon |N|}{2} \cdot \frac{2}{|N|}
= \epsilon
\]

Hence, for every \( \epsilon > 0 \), there exists a \( \delta > 0 \) such that if \( 0 < |x - c| < \delta \), then:

\[
\left| \frac{f(x)}{g(x)} - \frac{L}{M} \right| < \epsilon
\]

Thus, we conclude:
\[
\lim_{x \to c} \frac{f(x)}{g(x)} = \frac{L}{M}
\]

\end{proof}

\end{document}