Claim: lim x->a (a ⋅ f(x)) = a ⋅ lim f(x)

Proof



We will directly prove that lim af(x) = a lim f(x) using the ε–δ definition.

Since Lim f(x) = L, this is the same as saying Lim af(x) = a lim f(x) = aL.



\#1. Lim af(x) = aL:

Given for every ε>0, there exists some δ>0, such that if 0 < |x-a| < δ then |af(x) - aL| < ε.

Then we must find such a delta with the information given.



Suppose |af(x) - aL| < ε.

Then |a||f(x)-L| < e.

It follows |f(x)-L| < e/|a|.

So let δ = e/|a|.

Then |af(x) - aL| < e/|a|.

Such that |f(x)-L| < e as we neede to prove.





\#2 aLim f(x) = aL:

Given for every ε>0, there exists some δ>0, such that if 0 < |x-a| < δ then |a\[(f(x) - L]| < ε.


Consider aLim f(x) = aL.

We simply divide both sides of the equation by a.

Hence, Limf(x) = L

So let δ = e.

Then |f(x)-L| < e as we wanted to prove.



Thus, for every ε>0, there exists some δ>0, such that if 0 < |x-a| < δ then |a\[(f(x) - L]| < ε and |af(x) - aL| < ε.

Hence, we can conclude Lim af(x) = aLimf(x) = aL.



Q.E.D



